coq/theories/imp2asm/ImpToASMCodegenProofs.v
@@ -1,0 +1,151 @@
+Require Import impboot.utils.Core.
+Require Import impboot.utils.Env.
+Require Import impboot.utils.AppList.
+Require Import coqutil.Word.Interface.
+Require Import impboot.imp2asm.ImpToASMCodegen.
+Require Import impboot.imperative.ImpSyntax.
+Require Import impboot.imperative.ImpSemantics.
+Require Import impboot.assembly.ASMSyntax.
+Require Import impboot.assembly.ASMSemantics.
+
+(* Definitions of invariants and relations *)
+
+(* Checks that the sequence xs appears at index n in the code list. *)
+Fixpoint code_in (n : nat) (xs : list instr) (code : list instr) : Prop :=
+  match xs with
+  | [] => True
+  | x :: xs' => nth_error code n = Some x /\ code_in (n + 1) xs' code
+  end.
+
+(* Declares that there exists a starting position where the initial code fragment appears in instructions. *)
+Definition init_code_in (instructions : list instr) : Prop :=
+  exists start, code_in 0 (init start) instructions.
+
+(* Looks up the function with identifier n in a list of funcs and returns its parameters and body if found. *)
+Fixpoint lookup_fun (n : nat) (ds : list func) : option (list name * list cmd) :=
+  match ds with
+  | [] => None
+  | (Func fname params body) :: ds =>
+    if eqb fname n then Some (params, body)
+    else lookup_fun n ds
+  end.
+
+(* Finds the position of function n in f_lookup if it exists. *)
+Fixpoint lookup_f (n : nat) (fs : f_lookup) : option nat :=
+  match fs with
+  | [] => None
+  | (fname, pos) :: fs =>
+    if eqb fname n then Some pos
+    else lookup_f n fs
+  end.
+
+(* Ensures initial instructions are present and that each function in ds has its compiled form in instructions. *)
+Definition code_rel (fs : f_lookup) (ds : list func) (instructions : list instr) : Prop :=
+  init_code_in instructions /\
+  forall n params body,
+    lookup_fun n ds = Some (params, body) ->
+    exists pos,
+      lookup_f n fs = Some pos /\
+      code_in pos (flatten (fst (c_fundef (Func n params body) pos fs))) instructions.
+
+(* Establishes a relation between an imperative state and an ASM state, including code alignment and register setup. *)
+Definition state_rel (fs : f_lookup) (s : ImpSemantics.state) (t : ASMSemantics.state) : Prop :=
+  s.(ImpSemantics.input) = t.(input) /\
+  s.(ImpSemantics.output) = t.(output) /\
+  code_rel fs s.(funs) t.(instructions) /\
+  exists r14 r15,
+    t.(regs) R12 = Some (word.of_Z 16%Z) /\
+    t.(regs) R13 = Some (word.of_Z 0x7FFFFFFFFFFFFFFF%Z) /\
+    t.(regs) R14 = Some r14 /\
+    t.(regs) R15 = Some r15 /\
+    memory_writable r14 r15 t.(memory).
+
+(* Asserts that the given list of words matches the current stack content and RAX register in state t. *)
+Definition has_stack (t : ASMSemantics.state) (xs : list word_or_ret) : Prop :=
+  exists w ws,
+    xs = Word w :: ws /\
+    t.(regs) RAX = Some w /\
+    t.(stack) = ws.
+
+(* Constrains v to valid ranges and equates it with w in the context of ASM state t. *)
+Definition v_inv (t : ASMSemantics.state) (v : word64) (w : word64) : Prop :=
+  word.ltu v (word.of_Z (2 ^ 63)) = true /\ w = v.
+
+(* Checks that environment variables map to valid locations and values on the stack in the ASM state. *)
+Definition env_ok (env : IEnv.env) (vs : list (option nat)) (curr : list word_or_ret) (t : ASMSemantics.state) : Prop :=
+  List.length vs = List.length curr /\
+  forall n v,
+    IEnv.lookup env n = Some v ->
+    index_of n 0 vs < List.length curr /\
+    exists w,
+      nth_error curr (index_of n 0 vs) = Some (Word w) /\
+      v_inv t v w.
+
+(* Goals *)
+
+Definition goal :=
+  forall (env : IEnv.env) (s s1 : ImpSemantics.state) (c : cmd)
+         (res : result IEnv.env) (t : ASMSemantics.state)
+         (vs vs' : v_stack) (fs : f_lookup)
+         (asmc : asm_appl) (l1 : nat)
+         (curr rest : list word_or_ret),
+    EVAL_CMD s.(fuel) s env c = (res, s1) /\
+    res <> Err Crash /\
+    c_cmd c t.(pc) fs vs = (asmc, l1, vs') /\
+    state_rel fs s t /\
+    env_ok env vs curr t /\
+    has_stack t (curr ++ rest) /\
+    odd (List.length rest) = true /\
+    code_in t.(pc) (flatten asmc) t.(instructions)
+    ->
+    exists outcome,
+      (* TODO(kπ) we use an outer fuel for this *)
+      steps (State t, s.(fuel)) outcome /\
+      match outcome with
+      | (Halt ec output, ck) =>
+          prefix output (string_of_list_ascii s1.(ImpSemantics.output)) = true /\
+          ec = (word.of_Z 1)
+      | (State t1, ck) =>
+          state_rel fs s1 t1 /\
+          ck = s1.(fuel) /\
+          forall v,
+            res = Res v ->
+            exists w,
+              (* TODO(kπ) Do we need this? vvvvvv (probably in a different form?) *)
+              (* v_inv t1 v w /\ *)
+                has_stack t1 (Word w :: curr ++ rest) /\
+                t1.(pc) = l1
+      end.
+
+Definition goals :=
+  forall (env : IEnv.env) (cmds : list cmd) (s s1 : ImpSemantics.state)
+         (res : result IEnv.env) (t : ASMSemantics.state) (vs vs' : v_stack)
+         (fs : f_lookup) (asmcmds : asm_appl) (l1 : nat) (curr rest : list word_or_ret),
+    EVAL_CMDS s.(fuel) s env cmds = (res, s1) /\
+    res <> Err Crash /\
+    c_cmds cmds t.(pc) fs vs = (asmcmds, l1, vs') /\
+    state_rel fs s t /\
+    env_ok env vs curr t /\
+    has_stack t (curr ++ rest) /\
+    odd (List.length rest) = true /\
+    code_in t.(pc) (flatten asmcmds) t.(instructions)
+    ->
+    exists outcome,
+      steps (State t, s.(fuel)) outcome /\
+      match outcome with
+      | (Halt ec output, ck) =>
+          prefix output (string_of_list_ascii s1.(ImpSemantics.output)) = true /\
+          ec = word.of_Z 1
+      | (State t1, ck) =>
+          state_rel fs s1 t1 /\
+          ck = s1.(fuel) /\
+          forall vs',
+            res = Res vs' ->
+            exists ws,
+              (* TODO(kπ) Do we need this? vvvvvv (probably in a different form?) *)
+              (* Forall2 (v_inv t1) vs' ws /\ *)
+              has_stack t1 (map Word (rev ws) ++ curr ++ rest) /\
+              t1.(pc) = l1
+      end.
+
+
